simulation/correct_get_opcode.v
@@ -1,0 +1,129 @@
+From bpf.comm Require Import Regs State Monad.
+From bpf.monadicmodel Require Import Opcode rBPFInterpreter.
+From Coq Require Import List Lia ZArith.
+From compcert Require Import Integers Values Clight Memory.
+Import ListNotations.
+
+From bpf.proof Require Import Clightlogic MatchState CorrectRel CommonLemma CommonLemmaNat.
+
+From bpf.clight Require Import interpreter.
+
+(**
+Check get_opcode.
+get_opcode
+     : nat -> M opcode
+
+*)
+
+Section Get_opcode.
+
+  (** The program contains our function of interest [fn] *)
+  Definition p : Clight.program := prog.
+
+  (* [Args,Res] provides the mapping between the Coq and the C types *)
+  (* Definition Args : list CompilableType := [stateCompilableType].*)
+  Definition args : list Type := [(nat:Type)].
+  Definition res : Type := (opcode:Type).
+
+  (* [f] is a Coq Monadic function with the right type *)
+  Definition f : arrow_type args (M res) := get_opcode.
+
+  (* [fn] is the Cligth function which has the same behaviour as [f] *)
+  Definition fn: Clight.function := f_get_opcode.
+
+  (* [match_arg] relates the Coq arguments and the C arguments *)
+  Definition match_arg_list : DList.t (fun x => x -> val -> State.state -> Memory.Mem.mem -> Prop) args :=
+    (DList.DCons (stateless opcode_correct)
+                (DList.DNil _)).
+
+  (* [match_res] relates the Coq result and the C result *)
+  Definition match_res : res -> val -> State.state -> Memory.Mem.mem -> Prop := fun x v st m => opcode_step_correct x v.
+
+  Instance correct_function3_get_opcode : forall a, correct_function3 p args res f fn nil true match_arg_list match_res a.
+  Proof.
+    correct_function_from_body args.
+    correct_body.
+    (** how to use correct_* *)
+    unfold INV.
+    unfold f.
+    repeat intro.
+    get_invariant _op.
+
+    unfold stateless, opcode_correct in c0.
+    destruct c0 as (Hc_eq & Hc_range).
+    subst.
+
+    eexists. exists m, Events.E0.
+    unfold byte_to_opcode.
+    repeat split; unfold step2.
+    -
+      forward_star.
+      simpl.
+      rewrite Int.zero_ext_idem; [| lia].
+      rewrite Int.zero_ext_and; [| lia].
+      change (two_p 8 - 1)%Z with 255%Z.
+      unfold Int.and.
+      assert (Hc_z: (0 <= Z.of_nat c <= 255)%Z) by lia.
+      rewrite Int.unsigned_repr with (z:=Z.of_nat c); [| change Int.max_unsigned with 4294967295%Z; lia].
+      change (Int.unsigned (Int.repr 255)) with (Z.of_nat (Z.to_nat 255%Z)).
+      change (Int.unsigned (Int.repr 7)) with (Z.of_nat (Z.to_nat 7%Z)).
+      assert (Hzland: (0 <= Z.land (Z.of_nat c) (Z.of_nat (Z.to_nat 7)) <= 7)%Z). {
+        split.
+        rewrite Z.land_nonneg.
+        right; lia.
+        rewrite LemmaNat.land_land.
+        change (Z.to_nat 7%Z) with 7.
+        assert (Hnat_land: Nat.land c 7 <= 7) by (rewrite Nat.land_comm; rewrite LemmaNat.land_bound; lia).
+        lia.
+      }
+      rewrite Int.unsigned_repr; [| change Int.max_unsigned with 4294967295%Z; lia].
+      rewrite <- Z.land_assoc.
+      simpl.
+      forward_star.
+    -
+      unfold match_res, opcode_step_correct.
+      assert (Hc_le: 0 <= Nat.land c 7 <= 7). {
+        rewrite Nat.land_comm.
+        split. lia.
+        rewrite LemmaNat.land_bound.
+        lia.
+      }
+      change 7%Z with (Z.of_nat (Z.to_nat 7%Z)).
+      rewrite LemmaNat.land_land.
+      change (Z.to_nat 7) with 7.
+      remember (Nat.land c 7) as n.
+      destruct n eqn: Hld_imm; [ reflexivity |].
+      destruct n0 eqn: Hld_reg; [ reflexivity |].
+      destruct n1 eqn: Hst_imm; [ reflexivity |].
+      destruct n2 eqn: Hst_reg; [ reflexivity |].
+      destruct n3 eqn: Halu32; [ reflexivity |].
+      destruct n4 eqn: Hbranch; [ reflexivity |].
+      destruct n5 eqn: Hill.
+      exists 6; split ;[ reflexivity | intuition].
+      destruct n6 eqn: Halu64; [ reflexivity | lia].
+    - constructor.
+      simpl.
+      rewrite Int.zero_ext_and.
+      change (two_p 8 - 1)%Z with 255%Z.
+      unfold Int.and.
+      change (Int.unsigned (Int.repr 255)) with (Z.of_nat (Z.to_nat 255%Z)).
+      change 7%Z with (Z.of_nat (Z.to_nat 7%Z)) at 1.
+      assert (Hzland: (0 <= Z.land (Z.of_nat c) (Z.of_nat (Z.to_nat 7)) <= 7)%Z). {
+        split.
+        rewrite Z.land_nonneg.
+        right; lia.
+        rewrite LemmaNat.land_land.
+        change (Z.to_nat 7%Z) with 7.
+        assert (Hnat_land: Nat.land c 7 <= 7) by (rewrite Nat.land_comm; rewrite LemmaNat.land_bound; lia).
+        lia.
+      }
+      rewrite Int.unsigned_repr; [| change Int.max_unsigned with 4294967295%Z; lia].
+      rewrite <- Z.land_assoc.
+      simpl.
+      reflexivity.
+      lia.
+Qed.
+
+End Get_opcode.
+
+Existing Instance correct_function3_get_opcode.
